DynamoDbEncryptionMiddlewareInternal/src/DescribeTableTransform.dfy
@@ -1,0 +1,31 @@
+// Copyright Amazon.com Inc. or its affiliates. All Rights Reserved.
+// SPDX-License-Identifier: Apache-2.0
+
+include "DDBSupport.dfy"
+
+module DescribeTableTransform {
+  import opened DdbMiddlewareConfig
+  import opened DynamoDBMiddlewareSupport
+  import opened Wrappers
+  import DDB = ComAmazonawsDynamodbTypes
+  import opened AwsCryptographyDynamoDbEncryptionTypes
+  import EncTypes = AwsCryptographyDynamoDbItemEncryptorTypes
+  import Seq
+
+  method Input(config: Config, input: DescribeTableInputTransformInput)
+    returns (output: Result<DescribeTableInputTransformOutput, Error>)
+    ensures output.Success? && output.value.transformedInput == input.sdkInput
+  {
+    return Success(DescribeTableInputTransformOutput(transformedInput := input.sdkInput));
+  }
+
+  // TODO - implement this
+  method Output(config: Config, input: DescribeTableOutputTransformInput)
+    returns (output: Result<DescribeTableOutputTransformOutput, Error>)
+    requires ValidConfig?(config)
+    ensures ValidConfig?(config)
+    modifies ModifiesConfig(config)
+  {
+    return Success(DescribeTableOutputTransformOutput(transformedOutput := input.sdkOutput));
+  }
+}
